language/move-prover/bytecode-to-boogie/tests/goldenfiles/test-aborts-if.bpl
@@ -13,11 +13,11 @@ ensures old(b#Boolean(Boolean(i#Integer(x) <= i#Integer(y)))) ==> __abort_flag;
 
 {
     // declare local variables
-    var t2: Value; // IntegerType()
-    var t3: Value; // IntegerType()
-    var t4: Value; // BooleanType()
-    var t5: Value; // BooleanType()
-    var t6: Value; // IntegerType()
+    var __t2: Value; // IntegerType()
+    var __t3: Value; // IntegerType()
+    var __t4: Value; // BooleanType()
+    var __t5: Value; // BooleanType()
+    var __t6: Value; // IntegerType()
     var __tmp: Value;
     var __frame: int;
     var __saved_m: Memory;
@@ -113,9 +113,9 @@ ensures old(b#Boolean(Boolean(i#Integer(x) <= i#Integer(y)))) ==> __abort_flag;
 
 {
     // declare local variables
-    var t2: Value; // BooleanType()
-    var t3: Value; // BooleanType()
-    var t4: Value; // IntegerType()
+    var __t2: Value; // BooleanType()
+    var __t3: Value; // BooleanType()
+    var __t4: Value; // IntegerType()
     var __tmp: Value;
     var __frame: int;
     var __saved_m: Memory;
@@ -168,11 +168,11 @@ ensures old(b#Boolean(Boolean(i#Integer(x) < i#Integer(y)))) ==> __abort_flag;
 
 {
     // declare local variables
-    var t2: Value; // IntegerType()
-    var t3: Value; // IntegerType()
-    var t4: Value; // BooleanType()
-    var t5: Value; // BooleanType()
-    var t6: Value; // IntegerType()
+    var __t2: Value; // IntegerType()
+    var __t3: Value; // IntegerType()
+    var __t4: Value; // BooleanType()
+    var __t5: Value; // BooleanType()
+    var __t6: Value; // IntegerType()
     var __tmp: Value;
     var __frame: int;
     var __saved_m: Memory;
@@ -231,11 +231,11 @@ ensures old(b#Boolean(Boolean(i#Integer(x) <= i#Integer(y)))) ==> __abort_flag;
 
 {
     // declare local variables
-    var t2: Value; // IntegerType()
-    var t3: Value; // IntegerType()
-    var t4: Value; // BooleanType()
-    var t5: Value; // BooleanType()
-    var t6: Value; // IntegerType()
+    var __t2: Value; // IntegerType()
+    var __t3: Value; // IntegerType()
+    var __t4: Value; // BooleanType()
+    var __t5: Value; // BooleanType()
+    var __t6: Value; // IntegerType()
     var __tmp: Value;
     var __frame: int;
     var __saved_m: Memory;
@@ -294,11 +294,11 @@ ensures old(b#Boolean(Boolean(i#Integer(x) < i#Integer(y)))) ==> __abort_flag;
 
 {
     // declare local variables
-    var t2: Value; // IntegerType()
-    var t3: Value; // IntegerType()
-    var t4: Value; // BooleanType()
-    var t5: Value; // BooleanType()
-    var t6: Value; // IntegerType()
+    var __t2: Value; // IntegerType()
+    var __t3: Value; // IntegerType()
+    var __t4: Value; // BooleanType()
+    var __t5: Value; // BooleanType()
+    var __t6: Value; // IntegerType()
     var __tmp: Value;
     var __frame: int;
     var __saved_m: Memory;
@@ -357,11 +357,11 @@ ensures old(b#Boolean(Boolean(i#Integer(x) < i#Integer(y)))) ==> __abort_flag;
 
 {
     // declare local variables
-    var t2: Value; // IntegerType()
-    var t3: Value; // IntegerType()
-    var t4: Value; // BooleanType()
-    var t5: Value; // BooleanType()
-    var t6: Value; // IntegerType()
+    var __t2: Value; // IntegerType()
+    var __t3: Value; // IntegerType()
+    var __t4: Value; // BooleanType()
+    var __t5: Value; // BooleanType()
+    var __t6: Value; // IntegerType()
     var __tmp: Value;
     var __frame: int;
     var __saved_m: Memory;
@@ -413,23 +413,23 @@ procedure TestAbortIf_abort7_verify (x: Value, y: Value) returns ()
     call TestAbortIf_abort7(x, y);
 }
 
-procedure {:inline 1} TestAbortIf_abort8 (x: Value, y: Value) returns (ret0: Value)
+procedure {:inline 1} TestAbortIf_abort8 (x: Value, y: Value) returns (__ret0: Value)
 requires ExistsTxnSenderAccount(__m, __txn);
-ensures !__abort_flag ==> b#Boolean(Boolean(IsEqual(ret0, Boolean(true))));
+ensures !__abort_flag ==> b#Boolean(Boolean(IsEqual(__ret0, Boolean(true))));
 ensures old(!(b#Boolean(Boolean(i#Integer(x) < i#Integer(y)))) && (b#Boolean(Boolean(i#Integer(x) > i#Integer(y))))) ==> !__abort_flag;
 ensures old(b#Boolean(Boolean(i#Integer(x) < i#Integer(y)))) ==> __abort_flag;
 
 {
     // declare local variables
-    var t2: Value; // IntegerType()
-    var t3: Value; // IntegerType()
-    var t4: Value; // BooleanType()
-    var t5: Value; // BooleanType()
-    var t6: Value; // IntegerType()
-    var t7: Value; // IntegerType()
-    var t8: Value; // IntegerType()
-    var t9: Value; // IntegerType()
-    var t10: Value; // BooleanType()
+    var __t2: Value; // IntegerType()
+    var __t3: Value; // IntegerType()
+    var __t4: Value; // BooleanType()
+    var __t5: Value; // BooleanType()
+    var __t6: Value; // IntegerType()
+    var __t7: Value; // IntegerType()
+    var __t8: Value; // IntegerType()
+    var __t9: Value; // IntegerType()
+    var __t10: Value; // BooleanType()
     var __tmp: Value;
     var __frame: int;
     var __saved_m: Memory;
@@ -483,19 +483,19 @@ Label_7:
     __tmp := Boolean(IsEqual(GetLocal(__m, __frame + 8), GetLocal(__m, __frame + 9)));
     __m := UpdateLocal(__m, __frame + 10, __tmp);
 
-    ret0 := GetLocal(__m, __frame + 10);
+    __ret0 := GetLocal(__m, __frame + 10);
     return;
 
 Label_Abort:
     __abort_flag := true;
     __m := __saved_m;
-    ret0 := DefaultValue;
+    __ret0 := DefaultValue;
 }
 
-procedure TestAbortIf_abort8_verify (x: Value, y: Value) returns (ret0: Value)
+procedure TestAbortIf_abort8_verify (x: Value, y: Value) returns (__ret0: Value)
 {
     assume ExistsTxnSenderAccount(__m, __txn);
-    call ret0 := TestAbortIf_abort8(x, y);
+    call __ret0 := TestAbortIf_abort8(x, y);
 }
 
 procedure {:inline 1} TestAbortIf_abort9 (x: Value, y: Value) returns ()
@@ -506,11 +506,11 @@ ensures old(b#Boolean(Boolean(i#Integer(x) > i#Integer(y))) || b#Boolean(Boolean
 
 {
     // declare local variables
-    var t2: Value; // IntegerType()
-    var t3: Value; // IntegerType()
-    var t4: Value; // BooleanType()
-    var t5: Value; // BooleanType()
-    var t6: Value; // IntegerType()
+    var __t2: Value; // IntegerType()
+    var __t3: Value; // IntegerType()
+    var __t4: Value; // BooleanType()
+    var __t5: Value; // BooleanType()
+    var __t6: Value; // IntegerType()
     var __tmp: Value;
     var __frame: int;
     var __saved_m: Memory;
