language/move-prover/bytecode-to-boogie/tests/goldenfiles/test-func-call.bpl
@@ -6,13 +6,13 @@
 
 // ** functions of module TestFuncCall
 
-procedure {:inline 1} TestFuncCall_f (x: Value) returns (ret0: Value)
+procedure {:inline 1} TestFuncCall_f (x: Value) returns (__ret0: Value)
 requires ExistsTxnSenderAccount(__m, __txn);
 {
     // declare local variables
-    var t1: Value; // IntegerType()
-    var t2: Value; // IntegerType()
-    var t3: Value; // IntegerType()
+    var __t1: Value; // IntegerType()
+    var __t2: Value; // IntegerType()
+    var __t3: Value; // IntegerType()
     var __tmp: Value;
     var __frame: int;
     var __saved_m: Memory;
@@ -38,28 +38,28 @@ requires ExistsTxnSenderAccount(__m, __txn);
     if (__abort_flag) { goto Label_Abort; }
     __m := UpdateLocal(__m, __frame + 3, __tmp);
 
-    ret0 := GetLocal(__m, __frame + 3);
+    __ret0 := GetLocal(__m, __frame + 3);
     return;
 
 Label_Abort:
     __abort_flag := true;
     __m := __saved_m;
-    ret0 := DefaultValue;
+    __ret0 := DefaultValue;
 }
 
-procedure TestFuncCall_f_verify (x: Value) returns (ret0: Value)
+procedure TestFuncCall_f_verify (x: Value) returns (__ret0: Value)
 {
     assume ExistsTxnSenderAccount(__m, __txn);
-    call ret0 := TestFuncCall_f(x);
+    call __ret0 := TestFuncCall_f(x);
 }
 
-procedure {:inline 1} TestFuncCall_g (x: Value) returns (ret0: Value)
+procedure {:inline 1} TestFuncCall_g (x: Value) returns (__ret0: Value)
 requires ExistsTxnSenderAccount(__m, __txn);
 {
     // declare local variables
-    var t1: Value; // IntegerType()
-    var t2: Value; // IntegerType()
-    var t3: Value; // IntegerType()
+    var __t1: Value; // IntegerType()
+    var __t2: Value; // IntegerType()
+    var __t3: Value; // IntegerType()
     var __tmp: Value;
     var __frame: int;
     var __saved_m: Memory;
@@ -85,51 +85,51 @@ requires ExistsTxnSenderAccount(__m, __txn);
     if (__abort_flag) { goto Label_Abort; }
     __m := UpdateLocal(__m, __frame + 3, __tmp);
 
-    ret0 := GetLocal(__m, __frame + 3);
+    __ret0 := GetLocal(__m, __frame + 3);
     return;
 
 Label_Abort:
     __abort_flag := true;
     __m := __saved_m;
-    ret0 := DefaultValue;
+    __ret0 := DefaultValue;
 }
 
-procedure TestFuncCall_g_verify (x: Value) returns (ret0: Value)
+procedure TestFuncCall_g_verify (x: Value) returns (__ret0: Value)
 {
     assume ExistsTxnSenderAccount(__m, __txn);
-    call ret0 := TestFuncCall_g(x);
+    call __ret0 := TestFuncCall_g(x);
 }
 
-procedure {:inline 1} TestFuncCall_h (b: Value) returns (ret0: Value)
+procedure {:inline 1} TestFuncCall_h (b: Value) returns (__ret0: Value)
 requires ExistsTxnSenderAccount(__m, __txn);
 ensures old(!(b#Boolean(Boolean(false)))) ==> !__abort_flag;
 ensures old(b#Boolean(Boolean(false))) ==> __abort_flag;
 
 {
     // declare local variables
-    var t1: Value; // IntegerType()
-    var t2: Value; // IntegerType()
-    var t3: Value; // IntegerType()
-    var t4: Value; // BooleanType()
-    var t5: Value; // IntegerType()
-    var t6: Value; // IntegerType()
-    var t7: Value; // IntegerType()
-    var t8: Value; // IntegerType()
-    var t9: Value; // BooleanType()
-    var t10: Value; // IntegerType()
-    var t11: Value; // IntegerType()
-    var t12: Value; // BooleanType()
-    var t13: Value; // BooleanType()
-    var t14: Value; // BooleanType()
-    var t15: Value; // BooleanType()
-    var t16: Value; // IntegerType()
-    var t17: Value; // IntegerType()
-    var t18: Value; // BooleanType()
-    var t19: Value; // BooleanType()
-    var t20: Value; // BooleanType()
-    var t21: Value; // BooleanType()
-    var t22: Value; // IntegerType()
-    var t23: Value; // IntegerType()
+    var x: Value; // IntegerType()
+    var y: Value; // IntegerType()
+    var __t3: Value; // IntegerType()
+    var __t4: Value; // BooleanType()
+    var __t5: Value; // IntegerType()
+    var __t6: Value; // IntegerType()
+    var __t7: Value; // IntegerType()
+    var __t8: Value; // IntegerType()
+    var __t9: Value; // BooleanType()
+    var __t10: Value; // IntegerType()
+    var __t11: Value; // IntegerType()
+    var __t12: Value; // BooleanType()
+    var __t13: Value; // BooleanType()
+    var __t14: Value; // BooleanType()
+    var __t15: Value; // BooleanType()
+    var __t16: Value; // IntegerType()
+    var __t17: Value; // IntegerType()
+    var __t18: Value; // BooleanType()
+    var __t19: Value; // BooleanType()
+    var __t20: Value; // BooleanType()
+    var __t21: Value; // BooleanType()
+    var __t22: Value; // IntegerType()
+    var __t23: Value; // IntegerType()
     var __tmp: Value;
     var __frame: int;
     var __saved_m: Memory;
@@ -160,11 +160,11 @@ ensures old(b#Boolean(Boolean(false))) ==> __abort_flag;
     call __tmp := CopyOrMoveValue(GetLocal(__m, __frame + 1));
     __m := UpdateLocal(__m, __frame + 5, __tmp);
 
-    call t6 := TestFuncCall_f(GetLocal(__m, __frame + 5));
+    call __t6 := TestFuncCall_f(GetLocal(__m, __frame + 5));
     if (__abort_flag) { goto Label_Abort; }
-    assume IsValidU64(t6);
+    assume IsValidU64(__t6);
 
-    __m := UpdateLocal(__m, __frame + 6, t6);
+    __m := UpdateLocal(__m, __frame + 6, __t6);
 
     call __tmp := CopyOrMoveValue(GetLocal(__m, __frame + 6));
     __m := UpdateLocal(__m, __frame + 2, __tmp);
@@ -175,11 +175,11 @@ Label_8:
     call __tmp := CopyOrMoveValue(GetLocal(__m, __frame + 1));
     __m := UpdateLocal(__m, __frame + 7, __tmp);
 
-    call t8 := TestFuncCall_g(GetLocal(__m, __frame + 7));
+    call __t8 := TestFuncCall_g(GetLocal(__m, __frame + 7));
     if (__abort_flag) { goto Label_Abort; }
-    assume IsValidU64(t8);
+    assume IsValidU64(__t8);
 
-    __m := UpdateLocal(__m, __frame + 8, t8);
+    __m := UpdateLocal(__m, __frame + 8, __t8);
 
     call __tmp := CopyOrMoveValue(GetLocal(__m, __frame + 8));
     __m := UpdateLocal(__m, __frame + 2, __tmp);
@@ -236,17 +236,17 @@ Label_27:
     call __tmp := CopyOrMoveValue(GetLocal(__m, __frame + 2));
     __m := UpdateLocal(__m, __frame + 23, __tmp);
 
-    ret0 := GetLocal(__m, __frame + 23);
+    __ret0 := GetLocal(__m, __frame + 23);
     return;
 
 Label_Abort:
     __abort_flag := true;
     __m := __saved_m;
-    ret0 := DefaultValue;
+    __ret0 := DefaultValue;
 }
 
-procedure TestFuncCall_h_verify (b: Value) returns (ret0: Value)
+procedure TestFuncCall_h_verify (b: Value) returns (__ret0: Value)
 {
     assume ExistsTxnSenderAccount(__m, __txn);
-    call ret0 := TestFuncCall_h(b);
+    call __ret0 := TestFuncCall_h(b);
 }
